Preservation of typing by renaming

theories/Renamings.v
@@ -27,13 +27,50 @@ rcomp r1 r2 i := r2 (r1 i).
 Equations up_ren (r : ren) : ren :=
 up_ren r := rcons 0 (rcomp r rshift).
 
+Lemma up_ren_proper (r1 r2 : ren) :
+  r1 =₁ r2 -> up_ren r1 =₁ up_ren r2.
+Proof.
+  intros Hr [|i]; simpl. reflexivity.
+  unfold rcomp, rshift. f_equal. apply Hr.
+Qed.
+
+(* Eval compute in (fun ρ => up_ren ρ 1). *)
+
+Equations up_rens (k : nat) (ρ : ren) : ren :=
+up_rens 0 ρ := ρ ;
+up_rens (S k) ρ := up_ren (up_rens k ρ).
+
+Lemma up_rens_lt (i k : nat) (ρ : ren) :
+  i < k -> up_rens k ρ i = i.
+Proof.
+  intro. induction k in i, H |- *; simpl.
+  - lia.
+  - destruct i as [|i]. simpl. reflexivity.
+    simpl. unfold rcomp, rshift. f_equal. apply IHk. lia.
+Qed.
+
+Lemma up_rens_gt (i k : nat) (ρ : ren) :
+  i >= k -> up_rens k ρ i = (ρ (i - k)) + k.
+Proof.
+  induction k in i |- *; intros; simpl.
+  - transitivity (ρ (i - 0)). 2: lia. assert (i = i - 0) by lia. rewrite H0 at 1. reflexivity.
+  - destruct i as [|i]; simpl. lia.
+    unfold rcomp, rshift. rewrite IHk; lia.
+Qed.
+
+Lemma up_rens_add n m ρ :
+  up_rens n (up_rens m ρ) =₁ up_rens (n + m) ρ.
+Proof.
+  induction n; simpl. reflexivity.
+  apply up_ren_proper. assumption.
+Qed.
 (*********************************************************************************)
 (** *** Trivial properties of renamings. *)
 (*********************************************************************************)
 
 (** Pointwise equality for functions. *)
-Definition eq1 {A B} : relation (A -> B) := pointwise_relation _ eq.
-Notation "f =₁ g" := (eq1 f g) (at level 75).
+(* Definition eq1 {A B} : relation (A -> B) := pointwise_relation _ eq.
+Notation "f =₁ g" := (eq1 f g) (at level 75). *)
 
 Lemma eq1_refl {A B} {x : A -> B} : x =₁ x.
 Proof. reflexivity. Qed.
@@ -55,3 +92,18 @@ Proof. intros H1 H2 i. simp rcomp. now rewrite H1, H2. Qed.
 Lemma congr_up_ren {r r'} :
   r =₁ r' -> up_ren r =₁ up_ren r'.
 Proof. intros H. simp up_ren. apply congr_rcons. now apply congr_rcomp. Qed.
+
+Lemma up_ren_comp r1 r2 :
+  rcomp (up_ren r1) (up_ren r2) =₁ up_ren (rcomp r1 r2).
+Proof.
+  intros [|n]; unfold rcomp; reflexivity.
+Qed.
+
+Lemma up_rens_comp k r1 r2 :
+  rcomp (up_rens k r1) (up_rens k r2) =₁ up_rens k (rcomp r1 r2).
+Proof.
+  induction k in r1, r2 |- *; intro n; simpl.
+  - reflexivity.
+  - rewrite up_ren_comp. apply congr_up_ren.
+    apply IHk.
+Qed.
