utils/Functor.v
@@ -1,0 +1,76 @@
+From Utils Require Import Generalities.
+From Stdlib Require Import List. Import ListNotations.
+
+(* This files defines utils about functors *)
+Class FMap (F : Type -> Type) := fmap : forall {X Y : Type}, (X -> Y) -> (F X -> F Y).
+Arguments fmap (F) {_ _ _}.
+
+Class Functor (F : Type -> Type) `{FMap F} := {
+  func_id : forall {X : Type},
+    fmap F (fun x : X => x) =₁ (fun x => x);
+
+  func_comp : forall {X Y Z : Type} (f : X -> Y) (g : Y -> Z),
+    (fun x => fmap F g (fmap F f x)) =₁ fmap F (fun x => g (f x))
+}.
+
+(** Examples of functors **)
+(* Identity functor *)
+#[export] Instance FMapId : FMap (fun X : Type => X) :=
+  fun _ _ f => f.
+#[export] Instance FId : Functor (fun X => X).
+Proof.
+  constructor; unfold fmap; repeat intro; reflexivity.
+Qed.
+
+(* Constant functor *)
+#[export] Instance FMapConst (C : Type) : FMap (fun _ => C) :=
+  fun _ _ _ => (fun c => c).
+#[export] Instance FConst (C : Type) : Functor (fun _ => C).
+Proof.
+  constructor; unfold fmap; repeat intro; reflexivity.
+Qed.
+
+(* Lists *)
+#[export] Instance FMapList : FMap list := map.
+#[export] Instance Flist : Functor list.
+Proof.
+  constructor; unfold fmap, FMapList; repeat intro.
+  - apply map_id.
+  - induction a; simpl.
+    reflexivity.
+    rewrite IHa. reflexivity.
+Qed.
+
+(* Product of functors *)
+#[export] Instance FMapProd F G `{FMap F} `{FMap G} : FMap (fun X => (F X * G X)%type) :=
+  fun X Y (f : X -> Y) '(xf, xg) => (fmap F f xf, fmap G f xg).
+#[export] Instance FProf F G `{Functor F} `{Functor G} : Functor (fun X => (F X * G X)%type).
+Proof.
+  constructor; unfold fmap, FMapProd; repeat intro; destruct a as [xf xg].
+  - rewrite 2!func_id. reflexivity.
+  - rewrite 2!func_comp. reflexivity.
+Qed.
+
+(* Sanity check *)
+Goal Functor (fun X => (X*nat*X)%type). typeclasses eauto. Qed.
+
+(** Lifting of a predicate to a functor **)
+Class Lift (F : Type -> Type) := lift : forall X, (X -> Prop) -> (F X -> Prop).
+Arguments lift (F) {_ _}.
+
+(* We will see what axioms we need *)
+Class Predicator (F : Type -> Type) `{Lift F}
+:= {}.
+
+#[export] Instance LiftList : Lift list := Forall.
+#[export] Instance PList : Predicator list.
+Qed.
+
+#[export] Instance LiftId : Lift (fun X => X) := fun _ P => P.
+#[export] Instance PId : Predicator (fun X => X).
+Qed.
+
+#[export] Instance LiftProd F G `{Lift F} `{Lift G} : Lift (fun X => (F X * G X)%type) :=
+fun _ P '(xf, xg) => (lift F P xf) /\ (lift G P xg).
+#[export] Instance PProd F G `{Predicator F} `{Predicator G} : Predicator (fun X => (F X * G X)%type).
+Qed.
